induction results for contract morphisms and cleanup

execution/theories/ContractMorphisms.v
@@ -9,13 +9,13 @@ From Coq Require Import FunctionalExtensionality.
 From Coq Require Import Permutation.
 From Coq Require Import RelationClasses.
 From ConCert.Execution Require Import Blockchain.
+From ConCert.Execution Require Import ChainedList.
+From ConCert.Execution Require Import ContractCommon.
 From ConCert.Execution Require Import Serializable.
 From ConCert.Execution Require Import ResultMonad.
 From ConCert.Execution Require Import BuildUtils.
 From ConCert.Execution Require Import InterContractCommunication.
 From ConCert.Utils Require Import RecordUpdate.
-
-(* Axiom todo : string -> forall {A}, A. *)
 
 (* TODO USE `GENERALIZE VARIABLE` SYNTAX TO GET RID OF ALL THE IMPLICIT NOTATION *)
 
@@ -32,7 +32,6 @@ Definition uncurry_4 {A B C D E : Type} (f : A -> B -> C -> D -> E) : A * B * C 
 Section ContractMorphisms.
 Context { Base : ChainBase }.
 
-
 (** First, a definition of a Contract Morphism, which is a function between contracts *)
 Section MorphismDefinition.
 Context `{Serializable Msg}  `{Serializable Setup}  `{Serializable State}  `{Serializable Error}
@@ -48,8 +47,8 @@ Record InitCM (C : Contract Setup Msg State Error) (C' : Contract Setup' Msg' St
         (* proof of commutativity *)
         init_commutes : 
             forall x : Chain * ContractCallContext * Setup,
-                uncurry_3 C'.(init) (init_inputs x) = 
-                init_outputs (uncurry_3 C.(init) x) ;
+                uncurry_3 (init C') (init_inputs x) = 
+                init_outputs (uncurry_3 (init C) x) ;
     }.
 
 (** The receive component *)
@@ -63,8 +62,8 @@ Record RecvCM (C : Contract Setup Msg State Error) (C' : Contract Setup' Msg' St
         (* proof of commutativity *)
         recv_commutes : 
             forall (x : Chain * ContractCallContext * State * option Msg), 
-                uncurry_4 C'.(receive) (recv_inputs x) = 
-                recv_outputs (uncurry_4 C.(receive) x) ;
+                uncurry_4 (receive C') (recv_inputs x) = 
+                recv_outputs (uncurry_4 (receive C) x) ;
     }.
 
 (** The definition *)
@@ -147,7 +146,7 @@ Qed.
 (* an explicit construction *)
 Lemma init_commutes_id (C : Contract Setup Msg State Error) :
     init_morphs_commute 
-        C.(init) C.(init) 
+        (init C) (init C) 
         (id_fun (Chain * ContractCallContext * Setup)) 
         (id_fun (result State Error)).
 Proof. now intro. Qed.
@@ -162,7 +161,7 @@ Definition id_cm_init (C : Contract Setup Msg State Error) :
 
 Lemma recv_commutes_id (C : Contract Setup Msg State Error) :
     recv_morphs_commute 
-        C.(receive) C.(receive) 
+        (receive C) (receive C) 
         (id_fun (Chain * ContractCallContext * State * option Msg)) 
         (id_fun (result (State * list ActionBody) Error)).
 Proof. now intro. Qed.
@@ -184,10 +183,10 @@ End IdentityMorphism.
 
 (** Deriving equality of Contract Morphisms *)
 Section EqualityOfMorphisms.
-Context     { Setup Setup' Msg Msg' State State' Error Error' : Type }
-`{Serializable Msg}  `{Serializable Setup}  `{Serializable State}  `{Serializable Error}
-`{Serializable Msg'} `{Serializable Setup'} `{Serializable State'} `{Serializable Error'}
-{C : Contract Setup Msg State Error} {C' : Contract Setup' Msg' State' Error'}.
+Context { Setup Setup' Msg Msg' State State' Error Error' : Type }
+    `{Serializable Msg}  `{Serializable Setup}  `{Serializable State}  `{Serializable Error}
+    `{Serializable Msg'} `{Serializable Setup'} `{Serializable State'} `{Serializable Error'}
+    {C : Contract Setup Msg State Error} {C' : Contract Setup' Msg' State' Error'}.
 
 Lemma is_eq_cm :
     forall (f g : ContractMorphism C C'), 
@@ -253,8 +252,8 @@ Context { Setup Setup' Setup'' Msg Msg' Msg'' State State' State'' Error Error' 
 (** The Init component *)
 Lemma compose_commutes_init (g : ContractMorphism C' C'') (f : ContractMorphism C  C') :
     init_morphs_commute 
-        C.(init) 
-        C''.(init)
+        (init C) 
+        (init C'')
         (compose (init_inputs  C' C'' (init_cm g)) (init_inputs  C C' (init_cm f)))
         (compose (init_outputs C' C'' (init_cm g)) (init_outputs C C' (init_cm f))).
 Proof.
@@ -267,8 +266,8 @@ Qed.
 (** The Recv component *)
 Lemma compose_commutes_recv (g : ContractMorphism C' C'') (f : ContractMorphism C  C') :
     recv_morphs_commute 
-        C.(receive)
-        C''.(receive)
+        (receive C)
+        (receive C'')
         (compose (recv_inputs  C' C'' (recv_cm g)) (recv_inputs  C C' (recv_cm f)))
         (compose (recv_outputs C' C'' (recv_cm g)) (recv_outputs C C' (recv_cm f))).
 Proof.
@@ -300,18 +299,17 @@ Definition composition_cm (g : ContractMorphism C' C'') (f : ContractMorphism C 
 
 End MorphismComposition.
 
-Section CompositionEGs.
+Section MorphismCompositionResults.
 Context { Setup Setup' Setup'' Setup''' Msg Msg' Msg'' Msg''' 
-State State' State'' State''' 
-Error Error' Error'' Error''' : Type }
-`{Serializable Msg} `{Serializable Setup} `{Serializable State} `{Serializable Error}
-`{Serializable Msg'} `{Serializable Setup'} `{Serializable State'} `{Serializable Error'}
-`{Serializable Msg''} `{Serializable Setup''} `{Serializable State''} `{Serializable Error''}
-`{Serializable Msg'''} `{Serializable Setup'''} `{Serializable State'''} `{Serializable Error'''}
-{ C : Contract Setup Msg State Error } 
-{ C' : Contract Setup' Msg' State' Error' }
-{ C'' : Contract Setup'' Msg'' State'' Error'' }
-{ C''' : Contract Setup''' Msg''' State''' Error''' }.
+          State State' State'' State''' Error Error' Error'' Error''' : Type }
+    `{Serializable Msg} `{Serializable Setup} `{Serializable State} `{Serializable Error}
+    `{Serializable Msg'} `{Serializable Setup'} `{Serializable State'} `{Serializable Error'}
+    `{Serializable Msg''} `{Serializable Setup''} `{Serializable State''} `{Serializable Error''}
+    `{Serializable Msg'''} `{Serializable Setup'''} `{Serializable State'''} `{Serializable Error'''}
+    { C : Contract Setup Msg State Error } 
+    { C' : Contract Setup' Msg' State' Error' }
+    { C'' : Contract Setup'' Msg'' State'' Error'' }
+    { C''' : Contract Setup''' Msg''' State''' Error''' }.
 
 (** Composition with the Identity morphism is trivial *)
 Proposition composition_id_cm_left :
@@ -359,7 +357,7 @@ Proof.
             (composition_cm (composition_cm h g) f)).
 Qed.
 
-End CompositionEGs.
+End MorphismCompositionResults.
 
 
 (** We will treat various type of contract morphisms, starting with isomorphisms. *)
@@ -428,18 +426,16 @@ End IsomorphismDefinition.
 
 
 Section Isomorphisms.
-Context { Setup Setup' Setup'' Setup''' 
-        Msg   Msg'   Msg''   Msg''' 
-        State State' State'' State''' 
-        Error Error' Error'' Error''' : Type }
-        `{Serializable Msg} `{Serializable Setup} `{Serializable State} `{Serializable Error}
-        `{Serializable Msg'} `{Serializable Setup'} `{Serializable State'} `{Serializable Error'}
-        `{Serializable Msg''} `{Serializable Setup''} `{Serializable State''} `{Serializable Error''}
-        `{Serializable Msg'''} `{Serializable Setup'''} `{Serializable State'''} `{Serializable Error'''}
-        { C : Contract Setup Msg State Error } 
-        { C' : Contract Setup' Msg' State' Error' }
-        { C'' : Contract Setup'' Msg'' State'' Error'' }
-        { C''' : Contract Setup''' Msg''' State''' Error''' }.
+Context { Setup Setup' Setup'' Setup''' Msg Msg' Msg'' Msg''' State State' State'' State''' 
+            Error Error' Error'' Error''' : Type }
+    `{Serializable Msg} `{Serializable Setup} `{Serializable State} `{Serializable Error}
+    `{Serializable Msg'} `{Serializable Setup'} `{Serializable State'} `{Serializable Error'}
+    `{Serializable Msg''} `{Serializable Setup''} `{Serializable State''} `{Serializable Error''}
+    `{Serializable Msg'''} `{Serializable Setup'''} `{Serializable State'''} `{Serializable Error'''}
+    { C : Contract Setup Msg State Error } 
+    { C' : Contract Setup' Msg' State' Error' }
+    { C'' : Contract Setup'' Msg'' State'' Error'' }
+    { C''' : Contract Setup''' Msg''' State''' Error''' }.
 
 Definition contracts_isomorphic 
     (C : Contract Setup Msg State Error)
@@ -490,176 +486,47 @@ End Isomorphisms.
 
 (** Now, onto injections *)
 Section Injections.
+Context { Setup Setup' Msg Msg' State State' Error Error' : Type }
+    `{Serializable Msg}  `{Serializable Setup}  `{Serializable State}  `{Serializable Error}
+    `{Serializable Msg'} `{Serializable Setup'} `{Serializable State'} `{Serializable Error'}
+    {C : Contract Setup Msg State Error} {C' : Contract Setup' Msg' State' Error'}.
 
 Definition is_inj {A B : Type} (f : A -> B) : Prop := 
     forall (a a' : A), f a = f a' -> a = a'.
 
 Definition is_inj_cm 
-        { Setup Setup' Msg Msg' State State' Error Error' : Type }
-        `{Serializable Msg}  `{Serializable Setup}  `{Serializable State}  `{Serializable Error}
-        `{Serializable Msg'} `{Serializable Setup'} `{Serializable State'} `{Serializable Error'}
-        {C : Contract Setup Msg State Error} {C' : Contract Setup' Msg' State' Error'}
     (f : ContractMorphism C C') : Prop := 
     (* init morphisms inject *)
     is_inj (init_inputs  C C' (init_cm f)) /\
     (* recv morphisms inject *)
     is_inj (recv_inputs  C C' (recv_cm f)).
 
-Definition contract_embeds 
-        { Setup Setup' Msg Msg' State State' Error Error' : Type }
-        `{Serializable Msg}  `{Serializable Setup}  `{Serializable State}  `{Serializable Error}
-        `{Serializable Msg'} `{Serializable Setup'} `{Serializable State'} `{Serializable Error'}
-        (C1 : Contract Setup Msg State Error) (C2 : Contract Setup' Msg' State' Error') := 
-    exists (f : ContractMorphism C1 C2), is_inj_cm f.
+Definition contract_embeds : Prop := 
+    exists (f : ContractMorphism C C'), is_inj_cm f.
 
 End Injections.
 
 
 (** Finally, we treat surjections, or quotients *)
 Section Surjections.
+Context { Setup Setup' Msg Msg' State State' Error Error' : Type }
+    `{Serializable Msg}  `{Serializable Setup}  `{Serializable State}  `{Serializable Error}
+    `{Serializable Msg'} `{Serializable Setup'} `{Serializable State'} `{Serializable Error'}
+    {C : Contract Setup Msg State Error} {C' : Contract Setup' Msg' State' Error'}.
 
 Definition is_surj {A B : Type} (f : A -> B) : Prop := 
     forall (b : B), exists (a : A), f a = b.
 
-Definition is_surj_cm 
-        { Setup Setup' Msg Msg' State State' Error Error' : Type }
-        `{Serializable Msg}  `{Serializable Setup}  `{Serializable State}  `{Serializable Error}
-        `{Serializable Msg'} `{Serializable Setup'} `{Serializable State'} `{Serializable Error'}
-        {C : Contract Setup Msg State Error} {C' : Contract Setup' Msg' State' Error'}
-    (f : ContractMorphism C C') : Prop := 
+Definition is_surj_cm (f : ContractMorphism C C') : Prop := 
     (* init morphisms surject *)
     is_surj (init_inputs C C' (init_cm f)) /\
     (* recv morphisms surject *)
     is_surj (recv_inputs C C' (recv_cm f)).
 
-Definition contract_surjects 
-        { Setup Setup' Msg Msg' State State' Error Error' : Type }
-        `{Serializable Msg}  `{Serializable Setup}  `{Serializable State}  `{Serializable Error}
-        `{Serializable Msg'} `{Serializable Setup'} `{Serializable State'} `{Serializable Error'}
-        (C1 : Contract Setup Msg State Error) (C2 : Contract Setup' Msg' State' Error') := 
-    exists (f : ContractMorphism C1 C2), is_surj_cm f.
+Definition contract_surjects : Prop := 
+    exists (f : ContractMorphism C C'), is_surj_cm f.
 
 End Surjections.
-
-
-(** We have some interesting categorical properties, including the existence of a terminal
-    contract. (Note that we have not yet proved uniqueness of the terminal morphism.) *)
-Section TerminalContract.
-Import ListNotations.
-Set Nonrecursive Elimination Schemes.
-
-(** State *)
-Record Null_State := { null_state : unit }.
-
-(** Msg *)
-Inductive Null_Msg := 
-| null_msg (n : unit).
-
-(** Setup *)
-Definition Null_Setup := option unit.
-
-(* one canonical error message *)
-Definition Null_Error := unit.
-
-(** Init/Recv Functions *)
-Definition null_init 
-    (_ : Chain) 
-    (_ : ContractCallContext) 
-    (null_init : Null_Setup) : result Null_State Null_Error := 
-        match null_init with 
-        | Some _ => Ok {| null_state := tt |}
-        | None => Err tt
-        end.
-
-Definition null_recv
-    (_ : Chain) 
-    (_ : ContractCallContext) 
-    (_ : Null_State) 
-    (op_msg : option Null_Msg) : 
-    result (Null_State * list ActionBody) Null_Error := 
-        match op_msg with 
-        | Some _ => Ok ({| null_state := tt |}, [])
-        | None => Err tt
-        end.
-
-(** Derive [Serializable] instances for state and messages *)
-Global Instance Null_State_serializable : Serializable Null_State :=
-Derive Serializable Null_State_rect<Build_Null_State>.
-
-Global Instance Null_Msg_serializable : Serializable Null_Msg :=
-Derive Serializable Null_Msg_rect<null_msg>.
-
-(** the Terminal contract *)
-Definition null_contract : Contract Null_Setup Null_Msg Null_State Null_Error := 
-    build_contract null_init null_recv.
-
-(* prove that every contract has a morphism into the terminal contract *)
-Context 
-    { Setup Msg State Error : Type } 
-    `{Serializable Msg} `{Serializable Setup} `{Serializable State} `{Serializable Error}
-    { C : Contract Setup Msg State Error }.
-
-(* init morphisms *)
-Definition morph_init_i (x : Chain * ContractCallContext * Setup) : Chain * ContractCallContext * Null_Setup :=
-    let (x', s) := x in let (c, ctx) := x' in
-    match (C.(init) c ctx s) with 
-    | Ok  _ => (c, ctx, Some tt)
-    | Err _ => (c, ctx, None)
-    end.
-Definition morph_init_o (x : result State Error) : result Null_State Null_Error := 
-    match x with 
-    | Ok  _ => Ok {| null_state := tt |}
-    | Err _ => Err tt
-    end.
-Lemma null_init_commutes : init_morphs_commute C.(init) null_contract.(init) morph_init_i morph_init_o.
-Proof.
-    unfold init_morphs_commute. 
-    intro. destruct x as [x' s]. destruct x' as [c ctx]. simpl.
-    unfold uncurry_3. unfold null_init. unfold morph_init_o.
-    now destruct (init C c ctx s).
-Qed.
-
-(* recv morphisms *)
-Definition morph_recv_i (x : Chain * ContractCallContext * State * option Msg) : Chain * ContractCallContext * Null_State * option Null_Msg := 
-    let (x', op_msg) := x in
-    let (x'', st) := x' in 
-    let (c, ctx) := x'' in 
-    match (C.(receive) c ctx st op_msg) with 
-    | Ok  _ => (c, ctx, {| null_state := tt |}, (Some (null_msg tt)))
-    | Err _ => (c, ctx, {| null_state := tt |}, None)
-    end.
-Definition morph_recv_o (x : result (State * list ActionBody) Error) : result (Null_State * list ActionBody) Null_Error := 
-    match x with 
-    | Ok  _ => Ok ({| null_state := tt |}, [])
-    | Err _ => Err tt 
-    end.
-Lemma null_recv_commutes : recv_morphs_commute C.(receive) null_contract.(receive) morph_recv_i morph_recv_o.
-Proof.
-    unfold recv_morphs_commute. intro.
-    destruct x as [x' op_msg]. destruct x' as [x'' st]. destruct x'' as [c ctx]. simpl.
-    unfold uncurry_4. unfold null_recv. unfold morph_recv_o.
-    now destruct (receive C c ctx st op_msg).
-Qed.
-
-(* the terminal morphism *)
-Definition null_morphism : ContractMorphism C null_contract := 
-    let morph_init := {|
-        init_inputs   := morph_init_i ; 
-        init_outputs  := morph_init_o ;
-        init_commutes := null_init_commutes ;
-    |} in
-    let morph_recv := {|
-        recv_inputs   := morph_recv_i ;
-        recv_outputs  := morph_recv_o ; 
-        recv_commutes := null_recv_commutes ;
-    |} in {| 
-        cm_init := morph_init ; 
-        cm_recv := morph_recv ;
-    |}.
-
-(* TODO: Prove uniqueness *)
-
-End TerminalContract.
 
 
 (** The definition of contract morphisms is fairly general, and 
@@ -676,34 +543,34 @@ End TerminalContract.
     to allow for more contract morphisms.
 *)
 Section SimpleContractMorphism.
+Context { Setup Setup' Msg Msg' State State' Error Error' : Type }
+    `{Serializable Msg}  `{Serializable Setup}  `{Serializable State}  `{Serializable Error}
+    `{Serializable Msg'} `{Serializable Setup'} `{Serializable State'} `{Serializable Error'}.
 
-(** Some auxiliary functions for transforming component functions into morphism form *)
-Definition init_result_transform 
-        { State State' Error Error' : Type }
-    (state_morph : State -> State')
-    (error_morph : Error -> Error')
-    (x : result State Error) : result State' Error' :=
-    match x with 
-    | Ok t => Ok (state_morph t)
-    | Err e => Err (error_morph e)
-    end.
+Definition result_functor {T T' E E' : Type} : (T -> T') -> (E -> E') -> result T E -> result T' E' :=
+    fun (f_t : T -> T') (f_e : E -> E') (res : result T E) => 
+    match res with | Ok t => Ok (f_t t) | Err e => Err (f_e e) end.
 
-Definition recv_result_transform 
-        { State State' Error Error' : Type }
-    (state_morph : State -> State')
-    (error_morph : Error -> Error')
-    (x : result (State  * list ActionBody) Error) : result (State' * list ActionBody) Error' := 
-        match x with 
-        | Ok t => let '(st, l) := t in Ok (state_morph st, l)
-        | Err e => Err (error_morph e)
-        end.
+(** The definition of a simple contract morphism *)
+Record simple_cm 
+    (C : Contract Setup Msg State Error) (C' : Contract Setup' Msg' State' Error') := {
+    (* the components of a simple morphism f *)
+    msg_morph : Msg -> Msg' ;
+    setup_morph : Setup -> Setup' ;
+    state_morph : State -> State' ;
+    error_morph : Error -> Error' ;
+    (* coherence conditions *)
+    init_coherence : forall c ctx s, 
+        result_functor state_morph error_morph (init C c ctx s) = 
+        init C' c ctx (setup_morph s) ;
+    recv_coherence : forall c ctx st op_msg, 
+        result_functor (fun '(st, l) => (state_morph st, l)) error_morph (receive C c ctx st op_msg) = 
+        receive C' c ctx (state_morph st) (option_map msg_morph op_msg) ; }.
+
 
 (** We explicitly construct the components *)
 (* the init component *)
 Lemma init_commutes_simple 
-    { Setup Setup' Msg Msg' State State' Error Error' : Type }
-    `{Serializable Msg}  `{Serializable Setup}  `{Serializable State}  `{Serializable Error}
-    `{Serializable Msg'} `{Serializable Setup'} `{Serializable State'} `{Serializable Error'}
     {C1 : Contract Setup Msg State Error} 
     {C2 : Contract Setup' Msg' State' Error'}
     (* the components of f *)
@@ -712,25 +579,20 @@ Lemma init_commutes_simple
     (error_morph : Error -> Error')
     (* coherence conditions *)
     (init_coherence : forall c ctx s, 
-        (init_result_transform state_morph error_morph) ((init C1) c ctx s) = (init C2) c ctx (setup_morph s)) : 
+        result_functor state_morph error_morph (init C1 c ctx s) = init C2 c ctx (setup_morph s)) : 
     init_morphs_commute 
-        C1.(init) C2.(init)
+        (init C1) (init C2)
         (fun (x : Chain * ContractCallContext * Setup) => 
             let '(c, ctx, s) := x in (c, ctx, setup_morph s))
-        (init_result_transform state_morph error_morph).
+        (result_functor state_morph error_morph).
 Proof.
     unfold init_morphs_commute. 
     intro. destruct x. destruct p.
     unfold uncurry_3. simpl.
-    rewrite <- (init_coherence c c0 s).
-    unfold init_outputs. 
-    reflexivity.
+    now rewrite <- (init_coherence c c0 s).
 Qed.
 
 Definition simple_cm_init 
-    { Setup Setup' Msg Msg' State State' Error Error' : Type }
-    `{Serializable Msg}  `{Serializable Setup}  `{Serializable State}  `{Serializable Error}
-    `{Serializable Msg'} `{Serializable Setup'} `{Serializable State'} `{Serializable Error'}
     {C1 : Contract Setup Msg State Error} 
     {C2 : Contract Setup' Msg' State' Error'}
     (* the components of f *)
@@ -739,19 +601,16 @@ Definition simple_cm_init
     (error_morph : Error -> Error')
     (* coherence conditions *)
     (init_coherence : forall c ctx s, 
-        (init_result_transform state_morph error_morph) ((init C1) c ctx s) = (init C2) c ctx (setup_morph s)) : 
+        result_functor state_morph error_morph (init C1 c ctx s) = init C2 c ctx (setup_morph s)) : 
     InitCM C1 C2 := {| 
         init_inputs := (fun (x : Chain * ContractCallContext * Setup) => 
         let '(c, ctx, s) := x in (c, ctx, setup_morph s)) ; 
-        init_outputs := (init_result_transform state_morph error_morph) ; 
+        init_outputs := (result_functor state_morph error_morph) ; 
         init_commutes := init_commutes_simple setup_morph state_morph error_morph init_coherence ;
     |}.
 
 (* the recv component *)
 Lemma recv_commutes_simple 
-    { Setup Setup' Msg Msg' State State' Error Error' : Type }
-    `{Serializable Msg}  `{Serializable Setup}  `{Serializable State}  `{Serializable Error}
-    `{Serializable Msg'} `{Serializable Setup'} `{Serializable State'} `{Serializable Error'}
     {C1 : Contract Setup Msg State Error} 
     {C2 : Contract Setup' Msg' State' Error'}
     (* the components of f *)
@@ -760,26 +619,24 @@ Lemma recv_commutes_simple
     (error_morph : Error -> Error')
     (* coherence conditions *)
     (recv_coherence : forall c ctx st op_msg, 
-        (recv_result_transform state_morph error_morph) ((receive C1) c ctx st op_msg) = 
-        (receive C2) c ctx (state_morph st) (option_map msg_morph op_msg)) : 
+        result_functor (fun '(st, l) => (state_morph st, l)) error_morph (receive C1 c ctx st op_msg) 
+        = (receive C2) c ctx (state_morph st) (option_map msg_morph op_msg)) : 
     recv_morphs_commute
-        C1.(receive) C2.(receive)
+        (receive C1) (receive C2)
         (fun (x : Chain * ContractCallContext * State * option Msg) => 
             let '(c, ctx, st, op_msg) := x in (c, ctx, state_morph st, option_map msg_morph op_msg))
-        (recv_result_transform state_morph error_morph).
+        (result_functor (fun '(st, l) => (state_morph st, l)) error_morph).
 Proof.
     unfold recv_morphs_commute. 
-    intro. destruct x. repeat destruct p.
-    unfold uncurry_4. simpl.
-    rewrite <- (recv_coherence c c0 s o).
-    unfold recv_outputs.
-    reflexivity.
+    intro. 
+    destruct x. 
+    repeat destruct p.
+    unfold uncurry_4. 
+    simpl.
+    now rewrite <- recv_coherence.
 Qed.
 
 Definition simple_cm_recv 
-    { Setup Setup' Msg Msg' State State' Error Error' : Type }
-    `{Serializable Msg}  `{Serializable Setup}  `{Serializable State}  `{Serializable Error}
-    `{Serializable Msg'} `{Serializable Setup'} `{Serializable State'} `{Serializable Error'}
     {C1 : Contract Setup Msg State Error} 
     {C2 : Contract Setup' Msg' State' Error'}
     (* the components of f *)
@@ -788,22 +645,19 @@ Definition simple_cm_recv
     (error_morph : Error -> Error')
     (* coherence conditions *)
     (recv_coherence : forall c ctx st op_msg, 
-        (recv_result_transform state_morph error_morph) ((receive C1) c ctx st op_msg) = 
-        (receive C2) c ctx (state_morph st) (option_map msg_morph op_msg)) : 
+        result_functor (fun '(st, l) => (state_morph st, l)) error_morph (receive C1 c ctx st op_msg) 
+        = receive C2 c ctx (state_morph st) (option_map msg_morph op_msg)) : 
     RecvCM C1 C2 := {| 
         recv_inputs := 
             (fun (x : Chain * ContractCallContext * State * option Msg) => 
                 let '(c, ctx, st, op_msg) := x in (c, ctx, state_morph st, option_map msg_morph op_msg)) ; 
         recv_outputs := 
-            (recv_result_transform state_morph error_morph) ; 
+            (result_functor (fun '(st, l) => (state_morph st, l)) error_morph) ; 
         recv_commutes := recv_commutes_simple msg_morph state_morph error_morph recv_coherence ;
     |}.
 
 (* the simple contract morphism *)
-Definition simple_cm 
-    { Setup Setup' Msg Msg' State State' Error Error' : Type }
-    `{Serializable Msg}  `{Serializable Setup}  `{Serializable State}  `{Serializable Error}
-    `{Serializable Msg'} `{Serializable Setup'} `{Serializable State'} `{Serializable Error'}
+Definition simple_cm_construct
     {C1 : Contract Setup Msg State Error} 
     {C2 : Contract Setup' Msg' State' Error'}
     (* the components of f *)
@@ -813,10 +667,11 @@ Definition simple_cm
     (error_morph : Error -> Error')
     (* coherence conditions *)
     (init_coherence : forall c ctx s, 
-        (init_result_transform state_morph error_morph) ((init C1) c ctx s) = (init C2) c ctx (setup_morph s))
+        result_functor state_morph error_morph (init C1 c ctx s) = init C2 c ctx (setup_morph s))
     (recv_coherence : forall c ctx st op_msg, 
-        (recv_result_transform state_morph error_morph) ((receive C1) c ctx st op_msg) = 
-        (receive C2) c ctx (state_morph st) (option_map msg_morph op_msg)) : 
+        (result_functor (fun '(st, l) => (state_morph st, l)) error_morph) 
+            (receive C1 c ctx st op_msg) = 
+        receive C2 c ctx (state_morph st) (option_map msg_morph op_msg)) : 
     ContractMorphism C1 C2 := {| 
         cm_init := simple_cm_init setup_morph state_morph error_morph init_coherence ;
         cm_recv := simple_cm_recv msg_morph   state_morph error_morph recv_coherence ;
@@ -824,9 +679,6 @@ Definition simple_cm
 
 (* a predicate to indicate that a contract morphism is simple *)
 Definition is_simple_cm
-    { Setup Setup' Msg Msg' State State' Error Error' : Type }
-    `{Serializable Msg}  `{Serializable Setup}  `{Serializable State}  `{Serializable Error}
-    `{Serializable Msg'} `{Serializable Setup'} `{Serializable State'} `{Serializable Error'}
     {C1 : Contract Setup Msg State Error} 
     {C2 : Contract Setup' Msg' State' Error'} 
     (f : ContractMorphism C1 C2) : Prop := 
@@ -838,25 +690,15 @@ Definition is_simple_cm
     (error_morph : Error -> Error')
     (* coherence conditions *)
     (init_coherence : forall c ctx s, 
-        (init_result_transform state_morph error_morph) ((init C1) c ctx s) = (init C2) c ctx (setup_morph s))
+        result_functor state_morph error_morph (init C1 c ctx s) = init C2 c ctx (setup_morph s))
     (recv_coherence : forall c ctx st op_msg, 
-        (recv_result_transform state_morph error_morph) ((receive C1) c ctx st op_msg) = 
-        (receive C2) c ctx (state_morph st) (option_map msg_morph op_msg)),
-    f = simple_cm msg_morph setup_morph state_morph error_morph init_coherence recv_coherence.
-
-(* TODO *)
-(* a tactic for proving a morphism is simple 
-Ltac show_is_simple_cm := 
-    match goal with 
-    | |- is_simple_cm _ => 
-    end.
-*)
+        (result_functor (fun '(st, l) => (state_morph st, l)) error_morph) 
+            (receive C1 c ctx st op_msg) = 
+        receive C2 c ctx (state_morph st) (option_map msg_morph op_msg)),
+    f = simple_cm_construct msg_morph setup_morph state_morph error_morph init_coherence recv_coherence.
 
 (* a trivial lemma for convenience *)
 Lemma simple_cm_is_simple
-    { Setup Setup' Msg Msg' State State' Error Error' : Type }
-    `{Serializable Msg}  `{Serializable Setup}  `{Serializable State}  `{Serializable Error}
-    `{Serializable Msg'} `{Serializable Setup'} `{Serializable State'} `{Serializable Error'}
     {C1 : Contract Setup Msg State Error} 
     {C2 : Contract Setup' Msg' State' Error'}
     (* the components of f *)
@@ -866,11 +708,12 @@ Lemma simple_cm_is_simple
     {error_morph : Error -> Error'}
     (* coherence conditions *)
     {init_coherence : forall c ctx s, 
-        (init_result_transform state_morph error_morph) ((init C1) c ctx s) = (init C2) c ctx (setup_morph s)}
+        (result_functor state_morph error_morph) (init C1 c ctx s) = init C2 c ctx (setup_morph s)}
     {recv_coherence : forall c ctx st op_msg, 
-        (recv_result_transform state_morph error_morph) ((receive C1) c ctx st op_msg) = 
-        (receive C2) c ctx (state_morph st) (option_map msg_morph op_msg)} : 
-    is_simple_cm (simple_cm msg_morph setup_morph state_morph error_morph init_coherence recv_coherence).
+        (result_functor (fun '(st, l) => (state_morph st, l)) error_morph) 
+            (receive C1 c ctx st op_msg) = 
+        receive C2 c ctx (state_morph st) (option_map msg_morph op_msg)} : 
+    is_simple_cm (simple_cm_construct msg_morph setup_morph state_morph error_morph init_coherence recv_coherence).
 Proof. 
     unfold is_simple_cm.
     exists msg_morph. exists setup_morph. exists state_morph. 
@@ -878,15 +721,21 @@ Proof.
     auto.
 Qed.
 
-(* simple morphisms compose to simple morphisms *)
-Lemma composition_simple_cm
-    { Setup Setup' Setup'' Msg Msg' Msg'' State State' State'' Error Error' Error'' : Type }
+End SimpleContractMorphism.
+
+
+Section SimpleContractMorphism_Composition.
+
+Context { Setup Setup' Setup'' Msg Msg' Msg'' State State' State'' Error Error' Error'' : Type }
     `{Serializable Msg}    `{Serializable Setup}    `{Serializable State}    `{Serializable Error}
     `{Serializable Msg'}   `{Serializable Setup'}   `{Serializable State'}   `{Serializable Error'}
     `{Serializable Msg''}  `{Serializable Setup''}  `{Serializable State''}  `{Serializable Error''}
     { C : Contract Setup Msg State Error } 
     { C' : Contract Setup' Msg' State' Error' }
-    { C'' : Contract Setup'' Msg'' State'' Error'' } 
+    { C'' : Contract Setup'' Msg'' State'' Error'' }.
+
+(* simple morphisms compose to simple morphisms *)
+Lemma composition_simple_cm
     (g : ContractMorphism C' C'')
     (f : ContractMorphism C  C') :
     is_simple_cm g -> 
@@ -896,19 +745,9 @@ Proof.
     unfold is_simple_cm.
     intros g_simple f_simple.
     (* extract functions from g *)
-    destruct g_simple as [g_msg g_simple].
-    destruct g_simple as [g_setup g_simple].
-    destruct g_simple as [g_state g_simple].
-    destruct g_simple as [g_error g_simple].
-    destruct g_simple as [g_init g_simple].
-    destruct g_simple as [g_recv g_simple].
+    destruct g_simple as [g_msg [g_setup [g_state [g_error [g_init [g_recv g_simple]]]]]].
     (* extract functions from f *)
-    destruct f_simple as [f_msg f_simple].
-    destruct f_simple as [f_setup f_simple].
-    destruct f_simple as [f_state f_simple].
-    destruct f_simple as [f_error f_simple].
-    destruct f_simple as [f_init f_simple].
-    destruct f_simple as [f_recv f_simple].
+    destruct f_simple as [f_msg [f_setup [f_state [f_error [f_init [f_recv f_simple]]]]]].
     (* construct g \circ f *)
     exists (compose g_msg f_msg).
     exists (compose g_setup f_setup).
@@ -916,50 +755,73 @@ Proof.
     exists (compose g_error f_error).
     (* proof of init coherence *)
     assert (forall (c : Chain) (ctx : ContractCallContext) (s : Setup),
-        init_result_transform 
+        result_functor
             (compose g_state f_state)
             (compose g_error f_error) (init C c ctx s) =
-        init C'' c ctx (compose g_setup f_setup s)).
-    intros. simpl.
+        init C'' c ctx (compose g_setup f_setup s))
+    as gf_init.
+    { intros. simpl.
     rewrite <- g_init.
     rewrite <- f_init.
-    unfold init_result_transform. destruct (init C c ctx s); auto.
-    rename H11 into gf_init. 
-    exists gf_init. 
+    destruct (init C c ctx s); auto. }
+    exists gf_init.
     (* proof of recv coherence *)
     assert (forall (c : Chain) (ctx : ContractCallContext) (st : State) (op_msg : option Msg),
-        recv_result_transform 
-            (compose g_state f_state)
+        result_functor 
+            (fun '(st, l) => (compose g_state f_state st, l))
             (compose g_error f_error) (receive C c ctx st op_msg) =
-        receive C'' c ctx (compose g_state f_state st) (option_map (compose g_msg f_msg) op_msg)).
-    intros. simpl.
-    replace (option_map (compose g_msg f_msg) op_msg) with (option_map g_msg (option_map f_msg op_msg)).
-    rewrite <- g_recv.
-    rewrite <- f_recv.
-    unfold recv_result_transform. destruct (receive C c ctx st op_msg); simpl; auto. destruct t; auto.
-    destruct op_msg; auto.
-    rename H11 into gf_recv.
+        receive C'' c ctx (compose g_state f_state st) (option_map (compose g_msg f_msg) op_msg))
+    as gf_recv.
+    {   intros. simpl.
+        replace (option_map (compose g_msg f_msg) op_msg) with (option_map g_msg (option_map f_msg op_msg)).
+        rewrite <- g_recv.
+        rewrite <- f_recv.
+        destruct (receive C c ctx st op_msg); simpl; auto. 
+        destruct t; auto.
+        destruct op_msg; auto. }
     exists gf_recv.
     (* rewrite the LHS *)
-    rewrite g_simple. rewrite f_simple.
-    unfold composition_cm. unfold simple_cm.
+    rewrite g_simple. 
+    rewrite f_simple.
+    unfold composition_cm. 
+    unfold simple_cm_construct.
     apply is_eq_cm.
     - apply is_eq_cm_init. 
-        + simpl. apply functional_extensionality. 
-          intro. destruct x. destruct p. auto.
-        + simpl. apply functional_extensionality.
-          intro. destruct x; auto.
+        +   simpl. 
+            apply functional_extensionality. 
+            intro. 
+            destruct x. 
+            destruct p. 
+            auto.
+        +   simpl. 
+            apply functional_extensionality.
+            intro. 
+            destruct x; auto.
     - apply is_eq_cm_recv.
-        + simpl. apply functional_extensionality.
-          intro. destruct x. repeat destruct p. simpl. destruct o; auto.
-        + simpl. apply functional_extensionality.
-          intro. destruct x. destruct t. all: auto.
+        +   simpl. 
+            apply functional_extensionality.
+            intro. 
+            destruct x. 
+            repeat destruct p. 
+            simpl. 
+            destruct o; auto.
+        +   simpl. 
+            apply functional_extensionality.
+            intro. 
+            destruct x. 
+            destruct t. 
+            all: auto.
 Qed.
+
+End SimpleContractMorphism_Composition.
+
+
+Section IdSimple.
+Context { Setup Msg State Error : Type }
+    `{Serializable Msg}  `{Serializable Setup}  `{Serializable State} `{Serializable Error}.
 
 (* the identity is a simple morphism *)
 Lemma identity_simple 
-    { Setup Msg State Error : Type }
-    `{Serializable Msg}  `{Serializable Setup}  `{Serializable State} `{Serializable Error}
     (C : Contract Setup Msg State Error) : 
     is_simple_cm (id_cm C).
 Proof. 
@@ -969,36 +831,219 @@ Proof.
     exists (id_fun State).
     exists (id_fun Error).
     assert (forall (c : Chain) (ctx : ContractCallContext) (s : Setup),
-            init_result_transform (id_fun State) (id_fun Error) (init C c ctx s) =
-            init C c ctx (id_fun Setup s)).
-    intros. unfold init_result_transform. unfold id_fun; simpl. destruct (init C c ctx s); auto.
-    rename H3 into id_init.
+            result_functor (id_fun State) (id_fun Error) (init C c ctx s) =
+            init C c ctx (id_fun Setup s))
+    as id_init.
+    {   intros. 
+        unfold id_fun; simpl. 
+        now destruct (init C c ctx s). }
     exists id_init.
     assert (forall (c : Chain) (ctx : ContractCallContext) (st : State) (op_msg : option Msg),
-            recv_result_transform (id_fun State) (id_fun Error) (receive C c ctx st op_msg) =
-            receive C c ctx (id_fun State st) (option_map (id_fun Msg) op_msg)).
-    intros. unfold recv_result_transform. unfold option_map. unfold id_fun; simpl.
-    destruct op_msg.
-    destruct (receive C c ctx st (Some m)); auto. destruct t; auto.
-    destruct (receive C c ctx st None); auto. destruct t; auto.
-    rename H3 into id_recv.
+            result_functor (fun '(st, l) => (id_fun State st, l)) (id_fun Error) (receive C c ctx st op_msg) =
+            receive C c ctx (id_fun State st) (option_map (id_fun Msg) op_msg))
+    as id_recv.
+    {   intros. 
+        unfold option_map, id_fun.
+        destruct op_msg.
+        -   simpl.
+            now destruct (receive C c ctx st (Some m)).
+        -   simpl.
+            now destruct (receive C c ctx st None). }
     exists id_recv.
     (* prove that id_cm C is simple wrt the above definitions *)
-    unfold id_cm. unfold simple_cm.
+    unfold id_cm. 
+    unfold simple_cm_construct.
     apply is_eq_cm.
     - apply is_eq_cm_init.
-        + simpl. unfold id_fun. apply functional_extensionality. 
-          intro. destruct x. destruct p. auto.
-        + simpl. unfold id_fun. apply functional_extensionality. 
-          intro. destruct x; auto.
+        +   simpl. 
+            unfold id_fun. 
+            apply functional_extensionality. 
+            intro. 
+            destruct x. 
+            destruct p. 
+            auto.
+        +   simpl. 
+            unfold id_fun. 
+            apply functional_extensionality. 
+            intro. 
+            destruct x; auto.
     - apply is_eq_cm_recv.
-        + simpl. unfold id_fun. apply functional_extensionality. 
-          intro. destruct x. repeat destruct p. destruct o; auto.
-        + simpl. unfold id_fun. apply functional_extensionality. 
-          intro. destruct x; auto. destruct t. auto.
+        +   simpl. 
+            unfold id_fun. 
+            apply functional_extensionality. 
+            intro. 
+            destruct x. 
+            repeat destruct p. 
+            now destruct o.
+        +   simpl. 
+            unfold id_fun. 
+            apply functional_extensionality. 
+            intro. 
+            now destruct x; auto.
 Qed.
 
-End SimpleContractMorphism.
+End IdSimple.
+
+
+
+(** Morphism Induction: 
+    A proof technique for contract morphisms which allows us to carry the relationship
+    established by a contract morphism into contract_induction. *)
+Section MorphismInduction.
+
+(** Define the notion of a contract's trace, which is a chained list of successful
+    contract calls which mimics the blockchain. *)
+Section ContractTrace.
+    Context { Setup Msg State Error : Type }
+            `{Serializable Msg} `{Serializable Setup} `{Serializable State} `{Serializable Error}.
+
+    (* Notions of contract state stepping forward *)
+    Record ContractStep (C : Contract Setup Msg State Error)
+        (prev_cstate : State) (next_cstate : State) := 
+        build_contract_step {
+        seq_chain : Chain ;
+        seq_ctx : ContractCallContext ;
+        seq_msg : option Msg ;
+        seq_new_acts : list ActionBody ;
+        (* we can call receive successfully *)
+        recv_some_step : 
+            receive C seq_chain seq_ctx prev_cstate seq_msg = Ok (next_cstate, seq_new_acts) ;
+    }.
+
+    Definition ContractTrace (C : Contract Setup Msg State Error) := 
+        ChainedList State (ContractStep C).
+End ContractTrace.
+
+
+Context { Setup Setup' Msg Msg' State State' Error Error' : Type }
+    `{Serializable Msg}  `{Serializable Setup}  `{Serializable State}  `{Serializable Error}
+    `{Serializable Msg'} `{Serializable Setup'} `{Serializable State'} `{Serializable Error'}
+    {C : Contract Setup Msg State Error} {C' : Contract Setup' Msg' State' Error'}.
+
+(* A theorem to use if we are inducting on C *)
+(* - the relationship always exists with some parallel C' 
+        - rounding down/Uranium example. *)
+
+Theorem lef_cm_induction : 
+    (* forall simple morphism and reachable bstate, *)
+    forall (f : simple_cm C C') bstate caddr (trace : ChainTrace empty_state bstate),
+    (* where C is at caddr with state cstate, *)
+    env_contracts bstate caddr = Some (C : WeakContract) -> 
+    exists (cstate : State), 
+    contract_state bstate caddr = Some cstate /\
+    (* every reachable cstate of C corresponds to a reachable cstate' of C' on some chain ... *)
+    (exists (init_cstate' cstate' : State') (ctrace : ContractTrace C' init_cstate' cstate'),
+    (* 1. init_cstate' is a valid initial cstate of C'  *)
+    (exists init_chain init_ctx init_setup, init C' init_chain init_ctx init_setup = 
+        Ok init_cstate') /\
+    (* 2. cstate and cstate' are related by state_morph. *)
+    cstate' = state_morph C C' f cstate).
+Proof.
+    intros f_simple * c_at_caddr.
+    destruct f_simple as [msg_morph setup_morph state_morph error_morph init_coherence recv_coherence].
+    set (f := {|
+        msg_morph := msg_morph;
+        setup_morph := setup_morph;
+        state_morph := state_morph;
+        error_morph := error_morph;
+        init_coherence := init_coherence;
+        recv_coherence := recv_coherence
+      |}).
+    (* Prove by induction on the trace or by contract induction. *)
+    contract_induction; auto.
+    (* deployment *)
+    -   intros.
+        exists (state_morph result), (state_morph result).
+        exists clnil.
+        split; auto.
+        exists chain, ctx, (setup_morph setup).
+        rewrite <- (init_coherence chain ctx setup).
+        destruct (init C chain ctx setup); 
+        now try inversion init_some.
+    (* non-recursive call *)
+    -   intros.
+        destruct IH as [init_state' [cstate_prev' [prev_trace [init_correct IH]]]].
+        cbn in IH.
+        exists init_state', (state_morph new_state).
+        assert (ContractStep C' cstate_prev' (state_morph new_state))
+            as cstep.
+        {   set (seq_new_state := state_morph new_state).
+            set (seq_msg := option_map msg_morph msg).
+            apply (build_contract_step C' cstate_prev' seq_new_state chain ctx seq_msg new_acts).
+            (* now apply coherence *)
+            rewrite IH.
+            unfold seq_msg.
+            rewrite <- (recv_coherence chain ctx prev_state msg).
+            destruct (receive C chain ctx prev_state msg) eqn:H_rec;
+            now try inversion receive_some. }
+        exists (snoc prev_trace cstep).
+        split; auto.
+    (* recursive call *)
+    -   intros.
+        destruct IH as [init_state' [cstate_prev' [prev_trace [init_correct IH]]]].
+        cbn in IH.
+        exists init_state', (state_morph new_state).
+        assert (ContractStep C' cstate_prev' (state_morph new_state))
+            as cstep.
+        {   set (seq_new_state := state_morph new_state).
+            set (seq_msg := option_map msg_morph msg).
+            apply (build_contract_step C' cstate_prev' seq_new_state chain ctx seq_msg new_acts).
+            (* now apply coherence *)
+            rewrite IH.
+            unfold seq_msg.
+            rewrite <- (recv_coherence chain ctx prev_state msg).
+            destruct (receive C chain ctx prev_state msg) eqn:H_rec;
+            now try inversion receive_some. }
+        exists (snoc prev_trace cstep).
+        split; auto.
+    (* solve facts *)
+    -   intros.
+        solve_facts.
+Qed.
+
+
+(* A theorem to use if we are inducting on C' *)
+(* - if preimage, then relationship exists; OR reachable state => reachable state 
+        - upgradeability example
+        - backwards compatibility (inj)
+        - bug fix (surj) *)
+Theorem right_cm_induction:
+    forall (from to : State) (f : simple_cm C C'),
+    ContractTrace C from to ->
+    ContractTrace C' (state_morph C C' f from) (state_morph C C' f to).
+Proof.
+    intros * ctrace.
+    destruct f as [msg_morph setup_morph state_morph error_morph init_coherence recv_coherence].
+    set (f := {|
+        msg_morph := msg_morph;
+        setup_morph := setup_morph;
+        state_morph := state_morph;
+        error_morph := error_morph;
+        init_coherence := init_coherence;
+        recv_coherence := recv_coherence
+      |}).
+    cbn.
+    induction ctrace.
+    -   exact clnil.
+    -   assert (ContractStep C' (state_morph mid) (state_morph to))
+        as cstep.
+        {   destruct l as [s_chain s_ctx s_msg s_new_acts s_recv].
+            set (seq_msg := option_map msg_morph s_msg).
+            apply (build_contract_step C' (state_morph mid) (state_morph to) s_chain s_ctx seq_msg s_new_acts).
+            (* now apply coherence *)
+            unfold seq_msg.
+            rewrite <- (recv_coherence s_chain s_ctx mid s_msg).
+            destruct (receive C s_chain s_ctx mid s_msg) eqn:H_rec;
+            now try inversion s_recv. }
+        apply (snoc IHctrace cstep).
+Qed.
+
+
+(* TODO : Implications if there's a contract ISOmorphism. 
+    ... Can we compose these inductive rules?? *)
+
+
+End MorphismInduction.
 
 
 
