execution/theories/ContractSystems.v
@@ -20,8 +20,129 @@ Definition pair_fun2 {S T S' T' S'' T'' : Type}
     let (s,t) := x in let (s', t') := y in (f s s', g t t').
 
 
+Context {Base : ChainBase}.
+
+(** We have some interesting categorical properties, including the existence of a terminal
+    contract. (Note that we have not yet proved uniqueness of the terminal morphism.) *)
+Section TerminalContract.
+Import ListNotations.
+Set Nonrecursive Elimination Schemes.
+
+(** State *)
+Record Null_State := { null_state : unit }.
+
+(** Msg *)
+Inductive Null_Msg := 
+| null_msg (n : unit).
+
+(** Setup *)
+Definition Null_Setup := option unit.
+
+(* one canonical error message *)
+Definition Null_Error := unit.
+
+(** Init/Recv Functions *)
+Definition null_init 
+    (_ : Chain) 
+    (_ : ContractCallContext) 
+    (null_init : Null_Setup) : result Null_State Null_Error := 
+        match null_init with 
+        | Some _ => Ok {| null_state := tt |}
+        | None => Err tt
+        end.
+
+Definition null_recv
+    (_ : Chain) 
+    (_ : ContractCallContext) 
+    (_ : Null_State) 
+    (op_msg : option Null_Msg) : 
+    result (Null_State * list ActionBody) Null_Error := 
+        match op_msg with 
+        | Some _ => Ok ({| null_state := tt |}, [])
+        | None => Err tt
+        end.
+
+(** Derive [Serializable] instances for state and messages *)
+Global Instance Null_State_serializable : Serializable Null_State :=
+Derive Serializable Null_State_rect<Build_Null_State>.
+
+Global Instance Null_Msg_serializable : Serializable Null_Msg :=
+Derive Serializable Null_Msg_rect<null_msg>.
+
+(** The Terminal contract *)
+Definition null_contract : Contract Null_Setup Null_Msg Null_State Null_Error := 
+    build_contract null_init null_recv.
+
+(* prove that every contract has a morphism into the terminal contract *)
+Context 
+    { Setup Msg State Error : Type } 
+    `{Serializable Msg} `{Serializable Setup} `{Serializable State} `{Serializable Error}
+    { C : Contract Setup Msg State Error }.
+
+(* init morphisms *)
+Definition morph_init_i (x : Chain * ContractCallContext * Setup) : Chain * ContractCallContext * Null_Setup :=
+    let (x', s) := x in let (c, ctx) := x' in
+    match (C.(init) c ctx s) with 
+    | Ok  _ => (c, ctx, Some tt)
+    | Err _ => (c, ctx, None)
+    end.
+Definition morph_init_o (x : result State Error) : result Null_State Null_Error := 
+    match x with 
+    | Ok  _ => Ok {| null_state := tt |}
+    | Err _ => Err tt
+    end.
+Lemma null_init_commutes : init_morphs_commute C.(init) null_contract.(init) morph_init_i morph_init_o.
+Proof.
+    unfold init_morphs_commute. 
+    intro. destruct x as [x' s]. destruct x' as [c ctx]. simpl.
+    unfold uncurry_3. unfold null_init. unfold morph_init_o.
+    now destruct (init C c ctx s).
+Qed.
+
+(* recv morphisms *)
+Definition morph_recv_i (x : Chain * ContractCallContext * State * option Msg) : Chain * ContractCallContext * Null_State * option Null_Msg := 
+    let (x', op_msg) := x in
+    let (x'', st) := x' in 
+    let (c, ctx) := x'' in 
+    match (C.(receive) c ctx st op_msg) with 
+    | Ok  _ => (c, ctx, {| null_state := tt |}, (Some (null_msg tt)))
+    | Err _ => (c, ctx, {| null_state := tt |}, None)
+    end.
+Definition morph_recv_o (x : result (State * list ActionBody) Error) : result (Null_State * list ActionBody) Null_Error := 
+    match x with 
+    | Ok  _ => Ok ({| null_state := tt |}, [])
+    | Err _ => Err tt 
+    end.
+Lemma null_recv_commutes : recv_morphs_commute C.(receive) null_contract.(receive) morph_recv_i morph_recv_o.
+Proof.
+    unfold recv_morphs_commute. intro.
+    destruct x as [x' op_msg]. destruct x' as [x'' st]. destruct x'' as [c ctx]. simpl.
+    unfold uncurry_4. unfold null_recv. unfold morph_recv_o.
+    now destruct (receive C c ctx st op_msg).
+Qed.
+
+(* the terminal morphism *)
+Definition null_morphism : ContractMorphism C null_contract := 
+    let morph_init := {|
+        init_inputs   := morph_init_i ; 
+        init_outputs  := morph_init_o ;
+        init_commutes := null_init_commutes ;
+    |} in
+    let morph_recv := {|
+        recv_inputs   := morph_recv_i ;
+        recv_outputs  := morph_recv_o ; 
+        recv_commutes := null_recv_commutes ;
+    |} in {| 
+        cm_init := morph_init ; 
+        cm_recv := morph_recv ;
+    |}.
+
+(* TODO: Prove uniqueness *)
+
+End TerminalContract.
+
+
 Section ContractTransformations.
-Context { Base : ChainBase }.
 
 (** We define the product of two contracts *)
 Section ContractProducts.
@@ -165,7 +286,7 @@ End ContractSums.
 
 
 Section ContractSumsCorrect.
-Context     { Setup Setup' Setup'' Msg Msg' Msg'' State State' State'' Error Error' Error'' : Type }
+Context { Setup Setup' Setup'' Msg Msg' Msg'' State State' State'' Error Error' Error'' : Type }
     `{Serializable Msg} `{Serializable Setup} `{Serializable State} `{Serializable Error}
     `{Serializable Msg'} `{Serializable Setup'} `{Serializable State'} `{Serializable Error'}
     `{Serializable Msg''} `{Serializable Setup''} `{Serializable State''} `{Serializable Error''}
@@ -319,6 +440,11 @@ End PointedContract.
 End ContractTransformations.
 
 
+(** There have been some examples of contracts which aren't iso (counter, counter *2 for eg)
+    but would be for all reachable states.
+    In that eg, counter *2 always has an even number in storage, so there is an isomorphism
+    ** OF REACHABLE STATES **.
+    That's different from a contract isomorphism. *)
 
 
 
@@ -326,3 +452,363 @@ End ContractTransformations.
 
 
 
+
+
+(** TODO 
+
+Section MultiChainWeakEquivalences.
+
+Definition MultiChainState : Type := @ChainState Base1 * @ChainState Base2.
+Definition MultiChainStep (prev_multi_bstate : MultiChainState) (next_multi_bstate : MultiChainState) : Type := 
+        @ChainStep Base1 (fst prev_multi_bstate) (fst next_multi_bstate) +
+        @ChainStep Base2 (snd prev_multi_bstate) (snd next_multi_bstate) +
+       (@ChainStep Base1 (fst prev_multi_bstate) (fst next_multi_bstate) *
+        @ChainStep Base2 (snd prev_multi_bstate) (snd next_multi_bstate)).
+Definition MultiChainTrace := ChainedList MultiChainState MultiChainStep.
+
+(* multi-chain contract : Defn 6.3.2 *)
+
+
+(* multi-chain null contract *)
+
+(* multi-chain morphism *)
+Definition multichain_empty_state : MultiChainState := (empty_state, empty_state).
+
+Definition multichain_reachable (mstate : MultiChainState) : Prop := 
+    reachable (fst mstate) /\ reachable (snd mstate).
+
+(* A multi-chain morphism is a morphism of linked lists *)
+(* TODO restrict to reachability? *)
+Record MultiChainMorphism := build_multi_chain_morphism {
+    multichainstate_morph : MultiChainState -> MultiChainState ; 
+    multi_empty_fixpoint : 
+        multichainstate_morph multichain_empty_state = multichain_empty_state ; 
+    multichainstep_morph : 
+        forall mstate1 mstate2, 
+        MultiChainStep mstate1 mstate2 -> 
+        MultiChainStep (multichainstate_morph mstate1) (multichainstate_morph mstate2) ;
+}.
+
+(* Lemma : takes reachable states to reachable states *)
+(* TODO AFTER you sorted out contract morphisms *)
+
+(* composition of multi-chain morphisms *)
+(* an auxiliary lemma *)
+Lemma multichain_compose_fixpoint_result (mch1 mch2 : MultiChainMorphism) : 
+    compose (multichainstate_morph mch2) (multichainstate_morph mch1) multichain_empty_state =
+    multichain_empty_state.
+Proof. Admitted.
+
+(* composition of multi-chain morphisms *)
+Definition composition_mch (mch1 mch2 : MultiChainMorphism) : MultiChainMorphism := {| 
+    multichainstate_morph := 
+        compose (multichainstate_morph mch1) (multichainstate_morph mch2) ; 
+    multi_empty_fixpoint := multichain_compose_fixpoint_result mch2 mch1 ;
+    multichainstep_morph := (fun b1 b2 => 
+        compose 
+            (multichainstep_morph mch2 
+                (multichainstep_morph mch1 b1)
+                (multichainstep_morph mch2 b2))
+            (multichainstep_morph mch1 b1 b2)) ;
+|}.
+
+(* composition is associative *)
+Lemma composition_assoc_mch : forall mch1 mch2 mch3, 
+    composition_mch (composition_mch mch3 mch2) mch1 = 
+    composition_mch mch3 (composition_mch mch2 mch1).
+Proof. (* proof omitted *) Qed.
+
+(*** identity morphism *)
+(* an auxiliary lemma *)
+Lemma multi_empty_fixpoint_id : 
+    @id MultiChainState multichain_empty_state = multichain_empty_state.
+Proof. auto. Qed.
+
+(* the identity multi-chain morphism *)
+Definition id_mch : MultiChainMorphism := {| 
+    multichainstate_morph := @id MultiChainState ; 
+    multi_empty_fixpoint := multi_empty_fixpoint_id ;
+    multichainstep_morph := (fun b1 b2 => @id (MultiChainStep b1 b2)) ;
+|}.
+
+(* left and right composition results *)
+Lemma composition_mch_left : forall mch, composition_mch id_mch mch = mch.
+Proof. (* proof omitted *) Qed.
+
+Lemma composition_mch_right : forall mch, composition_mch mch id_mch = mch.
+Proof. (* proof omitted *) Qed.
+
+End MultiChainWeakEquivalences.
+
+
+
+Section WeakContractMorphisms.
+
+(* a weak morphism between a system of contracts and a monolithic contract *)
+
+
+(* THEN one corresponding to each of these constructions ^^ (with conditions on what's needed, e.g. account balances unchanged) *)
+
+End WeakContractMorphisms.
+
+
+Section ChainMorphisms.
+
+Record ChainMorphism := build_chain_morphism {
+    chainstate_morph : ChainState -> ChainState ; 
+    chainstep_morph : 
+        forall bstate1 bstate2, 
+        ChainStep bstate1 bstate2 -> 
+        ChainStep (chainstate_morph bstate1) (chainstate_morph bstate2) ;
+}.
+
+(* the identity chain morphism *)
+Definition id_chm : ChainMorphism := {| 
+    chainstate_morph := id_fun ChainState ; 
+    chainstep_morph := (fun b1 b2 => id_fun (ChainStep b1 b2)) ; |}.
+
+Definition composition_chm (chm2 chm1 : ChainMorphism) : ChainMorphism := {| 
+    chainstate_morph := compose (chainstate_morph chm2) (chainstate_morph chm1) ;
+    chainstep_morph  := (fun b1 b2 => 
+        compose 
+            (chainstep_morph chm2 
+                (chainstate_morph chm1 b1) 
+                (chainstate_morph chm1 b2)) 
+            (chainstep_morph chm1 b1 b2)) ;
+|}.
+
+Lemma composition_chm_left : forall chm, composition_chm id_chm chm = chm.
+Proof. 
+    intro. unfold composition_chm. 
+    destruct chm. f_equal; simpl.
+Qed.
+
+Lemma composition_chm_right : forall chm, composition_chm chm id_chm = chm.
+Proof. 
+    intro. unfold composition_chm. 
+    destruct chm. f_equal; simpl.
+Qed.
+
+Lemma composition_assoc_chm : forall chm1 chm2 chm3, 
+    composition_chm (composition_chm chm3 chm2) chm1 = 
+    composition_chm chm3 (composition_chm chm2 chm1).
+Proof.
+    intros. unfold composition_chm. f_equal.
+Qed.
+
+(* chain isomoprhisms, which are bisimulations of blockchains *)
+Definition is_iso_chm (f g : ChainMorphism) : Prop := 
+    composition_chm g f = id_chm /\ 
+    composition_chm f g = id_chm.
+
+End ChainMorphisms.
+
+(*  Some conditions under which a system of contracts can be 
+    contracted via a chain (e.g. bisimulated) *)
+
+Section SystemContraction.
+Import ListNotations.
+
+Definition cm_lift' 
+    { Setup Setup' Msg Msg' State State' Error Error' : Type }
+    `{Serializable Msg}  `{Serializable Setup}  `{Serializable State}  `{Serializable Error}
+    `{Serializable Msg'} `{Serializable Setup'} `{Serializable State'} `{Serializable Error'}
+    {C : Contract Setup Msg State Error} {C' : Contract Setup' Msg' State' Error'} : 
+    (f : ContractMorphism C C') -> ChainMorphism.
+
+
+(* the chainstate (cst) morphism : system to monolithic *)
+Definition cst_system_to_mono 
+    { Setup Setup' Msg Msg' State State' Error Error' : Type }
+    `{Serializable Msg}  `{Serializable Setup}  `{Serializable State}  `{Serializable Error}
+    `{Serializable Msg'} `{Serializable Setup'} `{Serializable State'} `{Serializable Error'}
+    {C : Contract Setup Msg State Error} {C' : Contract Setup' Msg' State' Error'}
+    (caddr1 caddr2 : Address)
+    (bstate : ChainState) : ChainState := 
+    {| chain_state_env :=
+       {| env_chain :=
+            {| chain_height := 0;
+               current_slot := 0;
+               finalized_height := 0; |};
+          env_account_balances a := 0%Z;
+          env_contract_states a := None;
+          env_contracts a := None; |};
+     chain_state_queue := [] |}.
+
+(* the chainstep (csp) morphism : system to monolithic *)
+Definition csp_system_to_mono
+
+(* the chain morphism (chm) : system to monolithic *)
+Definition chm_system_to_mono 
+
+
+
+
+
+Definition chm_mono_to_system
+
+
+Theorem system_contraction 
+        { Setup Setup' Msg Msg' State State' Error Error' : Type }
+        `{Serializable Msg}  `{Serializable Setup}  `{Serializable State}  `{Serializable Error}
+        `{Serializable Msg'} `{Serializable Setup'} `{Serializable State'} `{Serializable Error'}
+        {C : Contract Setup Msg State Error} {C' : Contract Setup' Msg' State' Error'} : 
+    forall bstate caddr1 caddr2, 
+    (* such that caddr1 is C and caddr2 is C' *)
+
+    (* the chain morphism defined above *)
+
+
+End SystemContraction.
+
+
+(** A weak equivalence of Environments and ChainStates *)
+Section ChainStateWeakEquivalence.
+(* SETTING:
+    - I have a system of contracts, which consists of: 
+        - a POINTED set of addresses, which is the point of contraction (perhaps define this yourself)
+    - I need to transform it into a disjoint sum of contracts living at one address
+    - And then prove a bisimulation
+*)
+
+Definition ActionWeakTransform (* 
+  - transforms actions into the contracts in the system into actions into the joined contract 
+  - this changes:
+    - from (modular => monolithic)
+    - to (modular => monolithic)
+    - msg (msg => inl msg or inr msg, etc) -- perhaps you define this when you define the contraction
+  - TODO what to do about deployments?
+*)
+
+Definition EnvironmentWeakEquiv (e1 e2 : Environment) 
+    (mon : (Address * WeakContract)) (* the monolithic contract *)
+    (sys : list (Address * WeakContract)) (* the system of contracts*) := 
+    build_env_weak_eq {
+        chain_weak_eq : 
+        (* we need to adjust chain height to account for deployments and, later, *) ;
+        account_balances_weak_eq : 
+            forall a,
+                (* if a not in list *)
+                (* then same *)
+                (* otherwise, sum of the list balances = the monolithic balance *) ;
+        contracts_weak_eq : 
+            forall a,
+                (* if a not in list *)
+                (* then same *)
+                (* otherwise, None in list, mon at mon_addr *) ;
+        contract_states_weak_eq : 
+            forall a,
+            (* if a not in list *)
+            (* then same *)
+            (* otherwise, None in list, mon's state at mon_addr *) ;
+    }.
+
+(*
+  - Chain : ?
+  - Balances : sum of balance of system should always equal balance of 
+  - (weak) Contracts : monolithic address has monolithic contract; each 
+  - States : states are none at old addresses, are the combined state at the pointed address 
+*)
+
+
+Definition ChainStateWeakEquiv (* 
+  - list Action : ?
+*)
+
+
+(*
+  - this is a NOTION of equivalence, parameterized over a system of contracts.
+  - you need to prove that this notion of equivalence is actually a BISIMULATION
+  - then provide sufficient conditions to achieve this ...
+     - the idea being that you take a system and combine it in any way listed above ^^.
+       then you have a single contract you can reason about.
+*)
+
+
+
+Context 
+    (* we can lift a morphism of contracts, parameterized by the morphpism f and the address of C1 *)
+    { Setup Setup' Msg Msg' State State' Error Error' : Type }
+    `{Serializable Msg}  `{Serializable Setup}  `{Serializable State}  `{Serializable Error}
+    `{Serializable Msg'} `{Serializable Setup'} `{Serializable State'} `{Serializable Error'}
+    {C1 : Contract Setup Msg State Error} {C2 : Contract Setup' Msg' State' Error'}
+    {f : ContractMorphism C1 C2}.
+
+Definition wc_dec_eq : forall w1 w2 : WeakContract, {w1 = w2} + {w1 <> w1} := todo "".
+Declare Scope wc_scope.
+Delimit Scope wc_scope with wc.
+Bind Scope wc_scope with WeakContract.
+Infix "=?" := wc_dec_eq (at level 70) : wc_scope.
+
+(* Given f, we can transform actions *)
+Definition action_transform { addrs : set Address } (native_env : Environment) (a : Action) : Action := {| 
+    act_origin := act_origin a ;
+    act_from := act_from a ;
+    act_body := 
+        match act_body a with 
+        (* contract calls into C1 change to calls into C2 *)
+        | act_call to amt msg => 
+            match env_contracts native_env to with 
+            | Some wc => 
+                if (wc =? contract_to_weak_contract C1)%wc
+                then act_call to amt msg
+                else act_body a
+            | None => act_body a
+            end
+        (* we deploy C2 instead of C1 *)
+        | act_deploy amt c setup => 
+            if (c =? contract_to_weak_contract C1)%wc
+            then act_deploy amt (contract_to_weak_contract C2) setup
+            else act_body a
+        (* all amounts stay the same, so we do not change transfers *)
+        | act_transfer _ _ => act_body a 
+        end
+|}.
+
+(* A morphism of Environments, parameterized implicitly over f by swapping out C2 for C1 *)
+Record EnvironmentMorphism (e1 e2 : Environment) := 
+    build_env_morphism {
+        chain_eq' : env_chain e1 = env_chain e2 ;
+        account_balances_eq' :
+            forall a, env_account_balances e1 a = env_account_balances e2 a ;
+        contracts_morph :
+            forall a, 
+                env_contracts e2 a = 
+                match env_contracts e1 a with 
+                | Some wc => 
+                    if (wc =? contract_to_weak_contract C1)%wc 
+                    then Some (contract_to_weak_contract C2) 
+                    else Some wc
+                | None => None 
+                end ;
+        contract_states_morph : 
+            forall a, 
+                env_contract_states e2 a = 
+                match env_contracts e1 a with 
+                | Some wc => 
+                    if (wc =? contract_to_weak_contract C1)%wc 
+                    then (option_fun (serialize_function state_morph)) (env_contract_states e1 a)
+                    else env_contract_states e1 a
+                | None => env_contract_states e1 a
+                end ;
+}.
+
+(* A morphism of ChainStates, parameterized implicitly over f *)
+Record ChainStateMorphism (cstate1 cstate2 : ChainState) := 
+    build_chainstate_morphism {
+        env_morph   : EnvironmentMorphism cstate1 cstate2 ;
+        queue_morph : chain_state_queue cstate2 = 
+                      List.map (action_transform cstate1) (chain_state_queue cstate1) ;
+    }.
+
+End ChainStateWeakEquivalence.
+
+
+Section WeakContractMorphismLift.
+
+
+
+End WeakContractMorphismLift.
+
+
+*)
